Subst lemma

TAPLFormalization/13-references/AST.lean
@@ -120,8 +120,13 @@ inductive SmallStep : State → State → Prop where
 
 infix:90 "~>" => SmallStep
 
-def TyCtx.insert_head (Γ : TyCtx) (ty : Typ) : TyCtx :=
-  fun x => if x = 0 then ty else Γ (x - 1)
+@[grind, simp]
+def TyCtx.shift (Γ : TyCtx) (c : ℕ) (S : Typ) : TyCtx :=
+  fun x => if x < c then Γ x else if x = c then S else Γ (x-1)
+
+@[grind, simp]
+def TyCtx.insert_head (Γ : TyCtx) (ty : Typ) : TyCtx := Γ.shift 0 ty
+
 
 @[grind]
 inductive Typing : TyCtx → Sgm → Term → Typ → Prop where
@@ -144,6 +149,58 @@ inductive Typing : TyCtx → Sgm → Term → Typ → Prop where
     Typing Γ σ t₁ (.ref T₁₁) →
     Typing Γ σ t₂ T₁₁ →
     Typing Γ σ (.assn t₁ t₂) (.unit)
+
+lemma shiftInCtx : ∀ t Γ σ T S c, Typing Γ σ t T → Typing (Γ.shift c S) σ (shift c 1 t) T := by
+  intro t
+  induction t with
+  | abs T_body body ih =>
+    intro Γ σ T S c h
+    cases h
+    rename_i R meow
+    rw[shift]
+    have ih := ih (Γ.insert_head T_body) σ R S (c+1) meow
+    have nika : ((Γ.insert_head T_body).shift (c + 1) S) = (Γ.shift c S).insert_head T_body := by
+      apply funext
+      intro x
+      by_cases x = 0 <;> by_cases x<c+1 <;> try simp_all
+      grind
+      grind
+    rw[nika] at ih
+    exact Typing.Abs ih
+  | app t₁ t₂ it₁ it₂ =>
+    intro Γ σ T S c h
+    cases h
+    rename_i R meow nya
+    rw[shift]
+    constructor
+    have it₂₂ := it₂ Γ σ (?app.App.T₁₁) S c meow
+    exact it₁ Γ σ (R.func T) S c nya
+    exact it₂ Γ σ R S c meow
+  | ref t it =>
+    intro Γ σ T S c h
+    cases h
+    rename_i R meow
+    rw[shift]
+    constructor
+    exact it Γ σ R S c meow
+  | deref t it =>
+    intro Γ σ T S c h
+    cases h
+    rename_i meow
+    rw[shift]
+    constructor
+    exact it Γ σ (.ref T) S c meow
+  | assn t₁ t₂ it₁ it₂ =>
+    intro Γ σ T S c h
+    cases h
+    rename_i T meow nya
+    rw[shift]
+    constructor
+    exact it₁ Γ σ (Typ.ref ?assn.Assign.T₁₁) S c meow
+    exact it₂ Γ σ T S c nya
+  | _ => grind
+
+lemma insert_head_ty : Typing Γ σ t T → Typing (Γ.insert_head S) σ (shift 0 1 t) T := by grind[shiftInCtx]
 
 def StoreWellTyped (Γ : TyCtx) (σ : Sgm) (μ : Store) : Prop :=
   ∀ l, match σ l, μ l with
@@ -179,32 +236,30 @@ lemma weakening : Typing Γ σ t T → σ'.extends σ → Typing Γ σ' t T := b
   intro t_ty sig_ext
   induction t_ty <;> try grind [Sgm.extends]
 
--- lemma insert_head_ty : Typing Γ σ t T → Typing (Γ.insert_head S) σ (shift 0 1 t) T := by
---   intro t_ty
---   induction t generalizing T <;> unfold TyCtx.insert_head <;> try grind [Typing, shift]
---   case app body arg body_ih arg_ih =>
---     rw [shift]
---     cases t_ty
---     rename_i T_in arg_ty body_ty
---     constructor
---     · exact body_ih body_ty
---     · exact arg_ih arg_ty
---   case abs T_body body ih =>
---     rw [shift]
---     cases t_ty
---     sorry
---   stop sorry
 
 lemma substitution : ∀ t s S T Γ x σ, (Typing (Γ.insert x S) σ t T ∧ Typing Γ σ s S → Typing Γ σ (sub' x s t) T) := by
-  sorry
-
--- s_ty : Typing Γ σ s S
--- body_ty : Typing (Γ.insert_head S) σ body T
--- Γ_eq' : Map.insert Γ' 0 S = Γ.insert_head S := sorry
--- ⊢ Typing Γ σ (Subst s body) T
-
--- lemma substitution : Typing Γ σ s S → Typing (Γ.insert_head S) σ body T → Typing Γ σ (Subst s body) T := by
---   sorry
+  intro t
+  induction t <;> try grind
+  case var n =>
+    intro s S T Γ x σ ⟨h₁, h₂⟩
+    by_cases n=x <;> cases h₁ <;> grind
+  case abs T t ih =>
+    intro s S T₁ Γ l σ ⟨abs_ty, s_ty⟩
+    cases abs_ty
+    rename_i R meow
+    rw [sub']
+    have : Typing (Γ.insert_head T) σ (sub' (l+1) (shift 0 1 s) t) R := by
+      have : Typing (Map.insert (Γ.insert_head T) (l+1) S) σ t R := by
+        have nika: Map.insert (Γ.insert_head T) (l+1) S = (TyCtx.insert_head (Map.insert Γ l S) T) := by
+          apply funext
+          intro x
+          by_cases x = 0 <;> by_cases x = l+1 <;>try simp_all
+          grind
+        rw[nika]
+        exact meow
+      have : Typing (Γ.insert_head T) σ (shift 0 1 s) S := by grind[shiftInCtx]
+      grind
+    grind
 
 @[simp, grind]
 lemma extends_insert : σ l = none → Sgm.extends (σ.insert l T) σ := by
@@ -245,14 +300,15 @@ lemma substitution' : Typing (Γ.insert_head S) σ body T
   → Typing Γ σ s S
   → Typing Γ σ (shiftDown (sub (shift 0 1 s) body)) T := by
   intro body_ty s_ty
-  induction body
-  case var n =>
+  induction body with
+  | var n =>
     cases n
     case zero =>
       cases body_ty
       simp [sub]
+      sorry
     sorry
-  sorry
+  | _ => sorry
 
 theorem preservation : Typing Γ σ t T → StoreWellTyped Γ σ μ
   → ⟨t, μ⟩ ~> ⟨t', μ'⟩
